fix duplicate definition problem

concurrency/framework/DiskExtern.h
@@ -78,7 +78,7 @@ namespace InstantiatedDiskInterface {
   inline Ptrs::Ptr get__event(IOCtx& ioctx) {
     struct io_event event;
     int status = io_getevents(*ioctx.ctx, 0, 1, &event, NULL);
-    if (status == 0) return Ptrs::__default::null_ptr;
+    if (status == 0) return Ptrs::null_ptr();
     assert (status == 1);
     assert (event.res > 0);
     iocb* i = event.obj;
