concurrency/framework/AIO.s.dfy
@@ -169,8 +169,8 @@ abstract module AIO(aioparams: AIOParams, ioifc: InputOutputIfc, ssm: DiskSSM(io
     iocb_ptr: Ptr,
     glinear fr: FinishedReq
   )
-  ensures iocb_ptr == nullptr ==> fr.FRNone?
-  ensures iocb_ptr != nullptr ==> (fr.FRWrite? || fr.FRRead?)
+  ensures iocb_ptr == nullptr() ==> fr.FRNone?
+  ensures iocb_ptr != nullptr() ==> (fr.FRWrite? || fr.FRRead?)
   ensures fr.FRWrite? ==>
     && fr.iocb.IocbWrite?
     && ctx.async_write_inv(iocb_ptr, fr.iocb, fr.data, fr.wg)
